tweaks after the lectures

Hoare3.v
@@ -18,6 +18,7 @@ Hint Rewrite aexp_pure_aeval bexp_pure_beval : opt.
 
 Section EqMR.
 
+
   (** *** Generalizing [EqM] *)
 
   (** Recall  [eqM : forall A, M A -> M A -> Prop] , in particular our insistance
@@ -29,27 +30,55 @@ Section EqMR.
   *)
 
 (* ----------------------------------------------------------------- *)
-(** *** More General Typeclass *)
+(** *** More General Typeclass of "Related" Computations *)
   (**
 
-Definition relationH A B := A -> B -> Prop
+Definition relH A B := A -> B -> Prop
 
 *)
 
-  Class EqMR (M : Type -> Type) : Type :=  {
-      eqMR : forall {A B : Type} (R : relationH A B), relationH (M A) (M B)
-  }.
+Class EqMR (M : Type -> Type) : Type :=  {
+    eqMR : forall {A B : Type} (R : relationH A B),
+      relationH (M A) (M B)
+}.
 
 End EqMR.
 
 (** Assuming [R : relationH A B] *)
 
-Notation "t1 ≈[ R ] t2" := (eutt R t1 t2) (at level 20).
+Notation "t1 ≈[ R ] t2" := (eutt R t1 t2)
+                             (at level 20).
 
-(** Note: we can _recover_ the ordinary [eqM] by instantiating [R] with [=] :
+(** [eutt R t1 t2] is weak bisimulation of trees whose leaves (i.e. the return nodes)
+   are related by [R].
 
-eqM := eqMR eq
-*)
+ *)
+
+Example eutt_trees : (Vis (Read "X") (fun n => Ret n))
+                       ≈[ lt ]
+                     (Vis (Read "X") (fun n => Ret (1 + n))).
+Proof.
+  apply eqit_Vis.
+  intros u.
+  apply eqit_Ret.
+  auto.
+Qed.
+
+(** Note: we can _recover_ the ordinary [eqM] by instantiating [R] with [eq]. *)
+
+(* ----------------------------------------------------------------- *)
+(** *** Intuition: [eqMR] *)
+
+(** The [R] parameter lets us specify a kind of "postcondition" that
+    lets is an assertion about the values returned by the computation.
+
+    In particular, if a tree is related to _itself_ with a given [R], i.e.:
+
+  t ≈[R] t
+
+    then we can think of the _diagonal_ of [R] as a predicate on the
+    returned values.
+ *)
 
 (* ----------------------------------------------------------------- *)
 (** *** Logical relation for (itree) [ret] *)
@@ -60,22 +89,41 @@ Check (@eutt_Ret).
 for this version, we have to show that it is.
 
     eqMR_Ret
-     : forall (E : Type -> Type) (R1 R2 : Type) (RR : relH R1 R2) (r1 : R1) (r2 : R2),
-      RR r1 r2 <-> Ret r1 ≈[ RR] Ret r2
+     : forall (E : Type -> Type)
+              (R1 R2 : Type)
+              (RR : relationH R1 R2)
+              (r1 : R1) (r2 : R2),
+
+      RR r1 r2
+      <->
+      Ret r1 ≈[RR] Ret r2
 *)
 
 (* ----------------------------------------------------------------- *)
 (** *** Logical relation for [bind] *)
 Check (@eutt_clo_bind).
+
 (** The generalization of [Proper] for [bind] looks like this:
 
 eqMR_bind
-     : forall (E : Type -> Type) (R1 R2 : Type) (RR : relH R1 R2) (U1 U2 : Type)
-         (UU : relH U1 U2) (t1 : itree E U1) (t2 : itree E U2) (k1 : U1 -> itree E R1)
-         (k2 : U2 -> itree E R2),
-       t1 ≈[ UU] t2 ->
+     : forall (E : Type -> Type)
+              (R1 R2 : Type) (RR : relationH R1 R2)
+              (U1 U2 : Type) (UU : relationH U1 U2)
+
+              (t1 : itree E U1)
+              (t2 : itree E U2)
+
+              (k1 : U1 -> itree E R1)
+              (k2 : U2 -> itree E R2),
+
+       (* logically-related initial trees *)
+       t1 ≈[UU] t2 ->
+
+       (* logically-related continuations *)
        (forall (u1 : U1) (u2 : U2), UU u1 u2 -> k1 u1 ≈[ RR] k2 u2) ->
-       (x <- t1;; k1 x) ≈[ RR] (x <- t2;; k2 x)
+
+       (* yield logically-related computations built with bind *)
+       (x <- t1;; k1 x) ≈[RR] (x <- t2;; k2 x)
 *)
 
 (* ----------------------------------------------------------------- *)
@@ -83,7 +131,7 @@ eqMR_bind
 
 (** [EqMR]
 
-- If [R] is a an equivalence then so is [≈[RR]]
+- If [R] is a an equivalence then so is [≈[R]]
 
 - Monotonicity: if [R1 ⊆ R2] then [≈[R1] ⊆ ≈[R2]]
 
@@ -95,14 +143,25 @@ Notation "a ∈ m" := (image m a)
 *)
 
 
+
 (* ----------------------------------------------------------------- *)
 (** *** Semantic Definition of Hoare Triples *)
 
+(** Predicates on the Imp memory state:
+
+Definition Assertion := mem -> Prop.
+*)
+
 Definition hoare_itree_triple (P:Assertion) (c:com) (Q:Assertion) :=
-  forall σ, P σ -> eutt (fun '(σ1,_) '(σ2,_) => σ1 = σ2 /\ Q σ1) (ℑ ⟦c⟧ σ) (ℑ ⟦c⟧ σ).
+  forall σ, P σ ->
+       (ℑ ⟦c⟧ σ)
+         ≈[(fun '(σ1,_) '(σ2,_) => σ1 = σ2 /\ Q σ1)]
+       (ℑ ⟦c⟧ σ).
 
 Notation "⦃ P ⦄  c  ⦃ Q ⦄" :=
-  (hoare_itree_triple P c Q) (at level 90, c custom com at level 99)
+  (hoare_itree_triple P c Q)
+
+    (at level 90, c custom com at level 99)
   : hoare_spec_scope.
 
 (* ----------------------------------------------------------------- *)
@@ -133,6 +192,9 @@ Proof.
   eapply H1; auto.
 Qed.
 
+(* ----------------------------------------------------------------- *)
+(** *** Hoare rules for Assignment *)
+
 Theorem hoare_itree_asgn : forall Q X a,
   ⦃Q [X |-> a]⦄ X := a ⦃Q⦄.
 Proof.
@@ -146,7 +208,9 @@ Qed.
 (** An alternative formulation that works better for forward reasoning. *)
 
 Theorem hoare_itree_asgn' : forall P X a,
-  ⦃P⦄ X := a ⦃ fun (σ:mem) => exists σ', σ = (X !-> (aeval σ' a) ; σ') /\ P σ' ⦄.
+    ⦃P⦄
+      X := a
+    ⦃ fun (σ:mem) => exists σ', σ = (X !-> (aeval σ' a) ; σ') /\ P σ' ⦄.
 Proof.
   unfold hoare_itree_triple.
   intros P X a σ H.
@@ -156,6 +220,9 @@ Proof.
   split. reflexivity.
   exists σ. split. reflexivity. assumption.
 Qed.
+
+(* ----------------------------------------------------------------- *)
+(** *** Hoare rules for Conditionals *)
 
 Theorem hoare_itree_if : forall P Q (b:bexp) c1 c2,
   ⦃ P /\ b ⦄ c1 ⦃Q⦄ ->
@@ -172,6 +239,9 @@ Proof.
   - apply H. intuition.
   - apply H0. intuition. simpl in H1. rewrite HB in H1. inversion H1.
 Qed.
+
+(* ----------------------------------------------------------------- *)
+(** *** Hoare rules for While Loop *)
 
 Theorem hoare_itree_while : forall P (b:bexp) c,
   ⦃P /\ b⦄ c ⦃P⦄ ->
@@ -211,6 +281,9 @@ Proof.
       estep. intuition.
       rewrite HB in H0. inversion H0.
 Qed.
+
+(* ----------------------------------------------------------------- *)
+(** *** Hoare rules for logical consequence *)
 
 Theorem hoare_itree_consequence_pre : forall (P P' Q : Assertion) c,
   ⦃P'⦄ c ⦃Q⦄ ->
@@ -267,6 +340,8 @@ Proof.
   - assumption.
 Qed.
 
+(* ----------------------------------------------------------------- *)
+(** *** Vacuous assertions *)
 Theorem hoare_itree_post_true : forall (P Q : Assertion) c,
   (forall st, Q st) ->
   ⦃P⦄ c ⦃Q⦄.
@@ -306,6 +381,8 @@ Proof.
   contradiction.
 Qed.
 
+(* ----------------------------------------------------------------- *)
+(** *** Hoare logic respects the semantics *)
 Lemma semantic_preservation : forall (P Q : Assertion) (c1 c2 : com),
     (forall σ, P σ -> ℑ⟦c1⟧σ ≈ ℑ⟦c2⟧σ) ->
     ⦃P⦄ c1 ⦃Q⦄ ->
@@ -319,6 +396,8 @@ Proof.
   apply HC1. assumption.
 Qed.
 
+(* ----------------------------------------------------------------- *)
+(** *** An Example *)
 Example hoare_itree_if_example :
   ⦃True⦄
     if X = 0
@@ -336,884 +415,5 @@ Proof.
     + assertion_auto'.
 Qed.
 
-(* ================================================================= *)
-(** ** Substitution *)
 
-Fixpoint substitute_aexp (x:string) (ax:aexp) (a:aexp) : aexp :=
-  match a with
-  | ANum n => a
-  | AId y => if String.eqb y x then ax else a
-  | <{ a1 + a2 }> => <{ (substitute_aexp x ax a1) + (substitute_aexp x ax a2) }>
-  | <{ a1 - a2 }> => <{ (substitute_aexp x ax a1) - (substitute_aexp x ax a2) }>
-  | <{ a1 * a2 }> => <{ (substitute_aexp x ax a1) * (substitute_aexp x ax a2) }>
-  end.
-
-Eval compute in (substitute_aexp X (<{ Y + 2}>) (<{ X + Z }>)).
-
-Lemma aexp_eval_semantics2 : forall a1 a2 σ,
-    (aeval σ a1 = aeval σ a2) <->
-      ℑ ⟦ a1 ⟧a σ ≈ ℑ ⟦ a2 ⟧a σ.
-Proof.
-  intros.
-  split.
-  - intros H.
-    norm.
-    rewrite H.
-    reflexivity.
-  - intros H.
-    unfold aexp_equiv in H.
-    do 2 rewrite aexp_pure_aeval in H.
-    apply eutt_Ret in H.
-    inversion H.
-    reflexivity.
-Qed.
-
-Lemma substitute_aexp_aeval : forall (x:string) ax a,
-  forall σ (EQ : aeval σ <{ x }> = aeval σ ax),
-    aeval σ a = aeval σ (substitute_aexp x ax a).
-Proof.
-  intros x ax a σ EQ.
-  induction a; simpl; auto.
-  destruct (String.eqb_spec x0 x).
-  - simpl in EQ. subst. assumption.
-  - reflexivity.
-Qed.
-
-Lemma substitute_aexp_semantic : forall (x:string) ax a,
-  forall σ (EQ: ℑ ⟦ <{ x }> ⟧a σ ≈ ℑ ⟦ ax ⟧a σ),
-    ℑ ⟦ a ⟧a σ ≈ ℑ ⟦ substitute_aexp x ax a ⟧a σ.
-Proof.
-  intros x ax a σ HEQ.
-  apply aexp_eval_semantics2.
-  intros. apply substitute_aexp_aeval.
-  apply aexp_eval_semantics2.
-  assumption.
-Qed.
-
-Lemma bexp_eval_semantics : forall b1 b2 σ,
-    (beval σ b1 = beval σ b2) <->
-      ℑ ⟦ b1 ⟧b σ ≈ ℑ ⟦ b2 ⟧b σ.
-Proof.
-  intros.
-  split.
-  - intros H.
-    norm.
-    rewrite H.
-    reflexivity.
-  - intros H.
-    unfold bexp_equiv in H.
-    do 2 rewrite bexp_pure_beval in H.
-    apply eutt_Ret in H.
-    inversion H.
-    reflexivity.
-Qed.
-
-Fixpoint substitute_bexp (x:string) (ax:aexp) (b:bexp) : bexp :=
-  match b with
-  | <{true}>      => b
-  | <{false}>     => b
-  | <{a1 = a2}>   => <{ (substitute_aexp x ax a1) = (substitute_aexp x ax a2) }>
-  | <{a1 <> a2}>   => <{ (substitute_aexp x ax a1) <> (substitute_aexp x ax a2) }>
-  | <{a1 <= a2}>  => <{ (substitute_aexp x ax a1) <= (substitute_aexp x ax a2) }>
-  | <{a1 > a2}>   => <{ (substitute_aexp x ax a1) > (substitute_aexp x ax a2) }>
-  | <{~ b1}>      => <{~ (substitute_bexp x ax b1) }>
-  | <{b1 && b2}>  => <{ (substitute_bexp x ax b1) && (substitute_bexp x ax b2) }>
-  end.
-
-Lemma substitute_bexp_beval : forall (x:string) ax b,
-  forall σ (EQ : aeval σ <{ x }> = aeval σ ax),
-    beval σ b = beval σ (substitute_bexp x ax b).
-Proof.
-  intros x ax b σ EQ.
-  induction b; simpl; try reflexivity.
-  - repeat rewrite <- (substitute_aexp_aeval x ax); auto.
-  - repeat rewrite <- (substitute_aexp_aeval x ax); auto.
-  - repeat rewrite <- (substitute_aexp_aeval x ax); auto.
-  - repeat rewrite <- (substitute_aexp_aeval x ax); auto.
-  - rewrite IHb. reflexivity.
-  - rewrite IHb1, IHb2. reflexivity.
-Qed.
-
-Lemma substitute_bexp_semantic : forall (x:string) ax b,
-  forall σ (EQ: ℑ ⟦ <{ x }> ⟧a σ ≈ ℑ ⟦ ax ⟧a σ),
-    ℑ ⟦ b ⟧b σ ≈ ℑ ⟦ substitute_bexp x ax b ⟧b σ.
-Proof.
-  intros x ax a σ HEQ.
-  apply bexp_eval_semantics.
-  intros. apply substitute_bexp_beval.
-  apply aexp_eval_semantics2.
-  assumption.
-Qed.
-
-Fixpoint contains (x:string) (a:aexp) : bool :=
-  match a with
-  | ANum n => false
-  | AId y => String.eqb y x
-  | <{ a1 + a2 }> => (contains x a1 || contains x a2)%bool
-  | <{ a1 - a2 }> => (contains x a1 || contains x a2)%bool
-  | <{ a1 * a2 }> => (contains x a1 || contains x a2)%bool
-  end.
-
-Lemma contains_false_equiv: forall (y:string) a,
-    contains y a = false ->
-    forall (σ:state) n, aeval σ a = aeval ( y !-> n ; σ ) a.
-Proof.
-  intros y.
-  induction a; intros HC σ m; simpl in *; try reflexivity.
-  - destruct (String.eqb_spec x y).
-    + inversion HC.
-    + rewrite t_update_neq; auto.
-  - apply Bool.orb_false_elim in HC.
-    destruct HC as [HA1 HA2].
-    auto.
-  - apply Bool.orb_false_elim in HC.
-    destruct HC as [HA1 HA2].
-    auto.
-  - apply Bool.orb_false_elim in HC.
-    destruct HC as [HA1 HA2].
-    auto.
-Qed.
-
-(** Because commands are not pure, we can't blindly substitute. *)
-
-Fixpoint substitute_com (x:string) (ax:aexp) (c:com) : (com * bool) :=
-  match c with
-  | <{ skip }> => (c, false)
-  | <{ y := a }> =>
-      let a' := substitute_aexp x ax a in
-      (<{ y := a' }>, ((y =? x)%string || contains y ax)%bool)
-  | <{ c1 ; c2 }> =>
-      let '(c1', stop) := substitute_com x ax c1 in
-      if stop
-      then (<{ c1' ; c2 }>, stop)
-      else
-        let '(c2', stop) := substitute_com x ax c2 in
-        (<{ c1' ; c2' }>, stop)
-  | <{ if b then c1 else c2 end }> =>
-      let '(c1', stop1) := substitute_com x ax c1 in
-      let '(c2', stop2) := substitute_com x ax c2 in
-      (<{ if (substitute_bexp x ax b) then c1' else c2' end }>, (stop1 || stop2)%bool)
-  | <{ while b do c end }> =>
-      let '(c', stop) := substitute_com x ax c in
-      if stop then (<{ while b do c end }>, true)
-      else (<{ while (substitute_bexp x ax b) do c' end}>, false)
-  end.
-
-(** Examples of when it is OK (or not) to substitute: *)
-Eval compute in substitute_com X 0 <{ Z := 3; Y := X + X ; Y := X }>.
-Eval compute in substitute_com X 0 <{ X := 3; X := X + X ; Y := X }>.
-
-(** Define an invariant that says when we can safely substitute the
-expression  <{ ax }> for <{ x }> in a state σ.  *)
-Definition subst_invariant x ax σ :=
-  aeval σ <{ x }> = aeval σ ax.
-
-(** Define the relational post condition for reasoning about the
-results of substitution. *)
-
-Definition post_condition x ax b (σ:state) :=
-  fun σ1 σ2 =>
-    σ1 = σ2
-    /\ (b = false -> (σ1 x = σ x /\ aeval σ ax = aeval σ1 ax /\ subst_invariant x ax σ1)).
-
-#[local]
- Instance post_condition_refl : forall x ax σ,
-    Reflexive (post_condition x ax true σ).
-Proof.
-  intros.
-  red.
-  intros.
-  unfold post_condition.
-  split. reflexivity. intros. inversion H.
-Qed.
-
-Lemma post_condition_mono : forall x ax σ st1 st2 b1 b2,
-    (b1 = true -> b2 = true) ->
-    post_condition x ax b1 σ st1 st2 ->
-    post_condition x ax b2 σ st1 st2.
-Proof.
-  intros.
-  unfold post_condition in *.
-  intuition.
-  - destruct b1.
-    + rewrite H in H0. inversion H0. reflexivity.
-    + apply H2. reflexivity.
-  - destruct b1.
-    + rewrite H in H0. inversion H0. reflexivity.
-    + apply H2. reflexivity.
-  - unfold subst_invariant in *. destruct b1.
-    + intuition. subst.  inversion H3.
-    + intuition.
-Qed.
-
-Lemma substitute_com_correct1 :
-  forall x ax c c' b
-    (HS: substitute_com x ax c = (c', b)),
-    forall σ (P: subst_invariant x ax σ),
-        eutt (prod_rel (post_condition x ax b σ) eq)
-             (ℑ ⟦c⟧ σ)
-             (ℑ ⟦c'⟧ σ).
-Proof.
-  intros x ax c.
-  induction c; intros; simpl in HS; inversion HS; subst; simpl; norm.
-  - apply eutt_Ret. unfold post_condition. auto.
-  - apply eutt_Ret.
-    simpl.
-    constructor; auto.
-    split; simpl; auto.
-    + rewrite <- substitute_aexp_aeval; auto.
-    + intros H.
-      destruct (String.eqb_spec x0 x).
-      * subst. simpl in H. inversion H.
-      * repeat split.
-       -- rewrite Bool.orb_false_l in H.
-          unfold subst_invariant in P.
-          apply t_update_neq.
-          assumption.
-       -- simpl in H.
-          erewrite contains_false_equiv. reflexivity.
-          assumption.
-       -- rewrite Bool.orb_false_l in H.
-          unfold subst_invariant in *.
-          erewrite <- contains_false_equiv.
-          erewrite <- contains_false_equiv; assumption.
-          cbn. apply eqb_neq. auto.
-  - destruct (substitute_com x ax c1).
-    specialize (IHc1 c b0 eq_refl σ P).
-    destruct b0.
-    + inversion HS. subst.
-      cbn.
-      norm.
-      eapply eutt_clo_bind.
-      apply IHc1.
-      intros u1 u2 HP.
-      destruct u1, u2, u, u0.
-      cbn.
-      destruct HP as [HM _].
-      destruct HM. simpl in H.
-      subst.
-      reflexivity.
-    + destruct (substitute_com x ax c2).
-      inversion HS. subst.
-      cbn.
-      norm.
-      eapply eutt_clo_bind.
-      apply IHc1.
-      intros u1 u2 HP.
-      destruct u1, u2, u, u0.
-      cbn.
-      destruct HP as [[HM H]].
-      simpl in HM.
-      subst.
-      specialize (H eq_refl).
-      destruct H as [HM HE].
-      simpl in *.
-      destruct HE as [HE H].
-      specialize (IHc2 c0 b eq_refl m0 H).
-      eapply eutt_subrel.
-      2: { apply IHc2. }
-      intros. unfold post_condition in H1.
-      inversion H1.
-      destruct a, u, b0, u.
-      constructor; auto.
-      unfold post_condition.
-      intuition.
-  - destruct (substitute_com x ax c1).
-    destruct (substitute_com x ax c2).
-    cbn.
-    inversion HS. subst.
-    cbn.
-    norm.
-    cbn.
-    rewrite <- substitute_bexp_beval; auto.
-    destruct (beval σ b).
-    + eapply eutt_subrel.
-      2:{ apply IHc1; auto. }
-      intros. constructor.
-      eapply post_condition_mono.
-      2: { apply H. }
-      intros. intuition.
-      inversion H; auto.
-    + eapply eutt_subrel.
-      2: { apply IHc2; auto. }
-      intros.
-      constructor.
-      eapply post_condition_mono.
-      2: { apply H. }
-      intros. intuition.
-      inversion H; auto.
-  - destruct (substitute_com x ax c).
-    destruct b1.
-    + inversion HS. subst.
-      reflexivity.
-    + inversion HS.
-      subst. clear HS H0.
-      cbn.
-      specialize (IHc c0 false eq_refl).
-      eapply eutt_subrel.
-      2 : { eapply eutt_interp_state_iter with (RS := post_condition x ax false σ)(RA := eq)(RB := eq).
-            intros.
-            unfold subst_invariant in *.
-            intuition. subst.
-            norm. cbn.
-            rewrite <- substitute_bexp_beval.
-            unfold post_condition in H.
-            intuition.  subst.
-            unfold subst_invariant in H3.
-            destruct (beval s2 b).
-            norm.
-            eapply eutt_clo_bind.
-            apply IHc. assumption.
-            intros. norm.  destruct u1. destruct u2.
-           apply eutt_Ret. cbn. apply prod_morphism. simpl.
-           apply fst_rel in H0. simpl in H0. unfold post_condition in H0. intuition.
-           subst.
-           unfold post_condition.
-           split; auto.
-           intros. intuition.
-           eapply snd_rel in H0. cbn. cbn in H0. subst. econstructor. reflexivity.
-           norm. apply eutt_Ret. apply prod_morphism. simpl.
-           unfold post_condition.
-           split; auto. cbn.  constructor. reflexivity.
-           unfold post_condition in H.
-           intuition.  subst. unfold subst_invariant in H3. subst.
-           intuition.
-           unfold subst_invariant in *.
-           unfold post_condition.
-           split; auto.
-           reflexivity. }
-      intros.
-      destruct a, b0.
-      cbn in *.
-      apply prod_morphism.
-      cbn.  intuition.  cbn. intuition.
-Qed.
-
-Fixpoint com_append (c1 c2 : com) : com :=
-  match c1 with
-  | <{ skip }> => c2
-  | <{ c11 ; c12}> => <{ c11 ; (com_append c12 c2) }>
-  | _ => <{ c1 ; c2 }>
-  end.
-
-(* TODO: This proof can be cleaned up using ImpEquiv *)
-Lemma com_append_correct : forall c1 c2,
-    com_append c1 c2 ≡ <{ c1 ; c2 }>.
-Proof.
-  induction c1; intro c2; simpl; try reflexivity.
-  - rewrite skipL_sound. reflexivity.
-  - rewrite seqA_sound. rewrite IHc1_2. reflexivity.
-Qed.
-
-#[global]
- Instance Proper_com_append: Proper (com_eq ==> com_eq ==> com_eq) com_append.
-Proof.
-  intros c11.
-  destruct c11; intros c12 EQ1 c21 c22 EQ2; simpl.
-  - rewrite com_append_correct. rewrite <- EQ1. rewrite skipL_sound. assumption.
-  - rewrite EQ1. rewrite com_append_correct. rewrite EQ2. reflexivity.
-  - rewrite com_append_correct. rewrite com_append_correct. rewrite <- EQ1.
-    rewrite seqA_sound. rewrite EQ2. reflexivity.
-  - rewrite com_append_correct. rewrite <- EQ1. rewrite EQ2. reflexivity.
-  - rewrite com_append_correct. rewrite <- EQ1. rewrite EQ2. reflexivity.
-Qed.
-
-Fixpoint com_assocR c : com :=
-  match c with
-  | <{ skip }> => c
-  | <{ y := a }> => c
-  | <{ c1 ; c2 }> =>
-      let c1' := com_assocR c1 in
-      let c2' := com_assocR c2 in
-      com_append c1' c2'
-  | <{ if b then c1 else c2 end }> =>
-      let c1' := com_assocR c1 in
-      let c2' := com_assocR c2 in
-      <{ if b then c1' else c2' end }>
-  | <{ while b do c end }> =>
-      let c' := com_assocR c in
-      <{ while b do c' end }>
-  end.
-
-Lemma com_assocR_correct : forall c,
-    c ≡ com_assocR c.
-Proof.
-  induction c; simpl; try reflexivity.
-  - rewrite <- IHc1. rewrite <- IHc2.
-    rewrite com_append_correct.
-    reflexivity.
-  - rewrite <- IHc1. rewrite <- IHc2.
-    reflexivity.
-  - rewrite <- IHc. reflexivity.
-Qed.
-
-Fixpoint propagate_com (c:com) : com :=
-  match c with
-  | <{ skip }> => c
-  | <{ y := a }> => c
-  | <{ y := a ; c2 }> =>
-      let c2' := propagate_com c2 in
-      if contains y a
-      then <{ y := a ; c2' }>
-      else <{ y := a;  fst (substitute_com y a c2') }>
-  | <{ c1 ; c2 }> =>
-      let c1' := propagate_com c1 in
-      let c2' := propagate_com c2 in
-      <{ c1' ; c2' }>
-  | <{ if b then c1 else c2 end }> =>
-      let c1' := propagate_com c1 in
-      let c2' := propagate_com c2 in
-      <{ if  b then c1' else c2' end }>
-  | <{ while b do c end }> =>
-      let c' := propagate_com c in
-      <{ while b do c' end }>
-  end.
-
-Lemma subst_invariant_good : forall (x:string) a σ,
-    contains x a = false ->
-    subst_invariant x a (x !-> aeval σ a; σ).
-Proof.
-  intros.
-  unfold subst_invariant.
-  eapply contains_false_equiv in H.
-  rewrite <- H.
-  symmetry.
-  simpl.
-  rewrite t_update_eq.
-  reflexivity.
-Qed.
-
-Lemma substitute_com_subst : forall c x a σ,
-    contains x a = false ->
-    ℑ ⟦ c ⟧ (x !-> aeval σ a; σ) ≈ ℑ ⟦ fst (substitute_com x a c) ⟧ (x !-> aeval σ a; σ).
-Proof.
-  intros.
-  destruct (substitute_com x a c) eqn:HS.
-  simpl.
-  apply substitute_com_correct1 with (σ := (x !-> aeval σ a; σ)) in HS.
-  eapply eutt_subrel.
-  2: { apply HS. }
-  intros.
-  destruct a0, u, b0, u.
-  inversion H0; clear H0.
-  unfold post_condition in fst_rel.
-  simpl in *.
-  intuition. subst. tauto.
-  apply subst_invariant_good.
-  assumption.
-Qed.
-
-Lemma propagate_com_sound : forall c,
-    c ≊ (propagate_com c).
-Proof.
-  induction c.
-  - simpl. reflexivity.
-  - simpl. reflexivity.
-  - simpl.
-    destruct c1.
-    + simpl. rewrite <- IHc2. reflexivity.
-    + destruct (contains x a) eqn:H.
-      * rewrite <- IHc2. reflexivity.
-      * intro.
-        cbn.
-        norm.
-        cbn.
-        eapply transitivity.
-        apply IHc2.
-        apply substitute_com_subst.
-        assumption.
-    + rewrite <- IHc1. rewrite <- IHc2. reflexivity.
-    + simpl in *.
-      rewrite IHc1.
-      rewrite <- IHc2.
-      reflexivity.
-    + simpl. rewrite <- IHc1. rewrite <- IHc2. reflexivity.
-  - simpl. rewrite <- IHc1. rewrite <- IHc2. reflexivity.
-  - simpl. rewrite <- IHc. reflexivity.
-Qed.
-
-Definition example : com :=
-  <{ X := 4 + 5;
-     Y := X;
-     if ((X - Y) = (2 + 4)) then skip
-     else Y := X end;
-     if (0 <= (4 - (2 + 1))) then Y := 0
-     else skip end;
-     while (Y = 0) do
-             X := X + 1
-             end
-    }>.
-
-Eval compute in fold_constants_com (propagate_com example).
-
-Example correct: example ≊ (fold_constants_com (propagate_com example)).
-Proof.
-  rewrite fold_constants_com_sound.
-  apply propagate_com_sound.
-Qed.
-
-Fixpoint loop_unroll_while (n:nat) (b:bexp) (c:com) : com :=
-  match n with
-  | 0 => <{ while b do c end }>
-  | S n => <{ if b then c ; (loop_unroll_while n b c) else skip end }>
-  end.
-
-Lemma loop_unroll_sound : forall (n:nat) (b:bexp) (c:com),
-    <{ while b do c end }> ≡ loop_unroll_while n b c.
-Proof.
-  induction n; intros; simpl.
-  - reflexivity.
-  - rewrite <- IHn.
-    apply loop_unroll1_sound_strong.
-Qed.
-
-Fixpoint loop_unroll_com n (c:com) : com :=
-  match c with
-  | <{ skip }> => c
-  | <{ y := a }> => c
-  | <{ c1 ; c2 }> =>
-      let c1' := loop_unroll_com n c1 in
-      let c2' := loop_unroll_com n c2 in
-      <{ c1' ; c2' }>
-  | <{ if b then c1 else c2 end }> =>
-      let c1' := loop_unroll_com n c1 in
-      let c2' := loop_unroll_com n c2 in
-      <{ if  b then c1' else c2' end }>
-  | <{ while b do c end }> =>
-      loop_unroll_while n b c
-  end.
-
-Lemma loop_unroll_com_sound : forall n c,
-    c ≊ (loop_unroll_com n c).
-Proof.
-  induction c.
-  - simpl. reflexivity.
-  - simpl. reflexivity.
-  - simpl. rewrite <- IHc1. rewrite <- IHc2. reflexivity.
-  - simpl. rewrite <- IHc1. rewrite <- IHc2. reflexivity.
-  - simpl. unfold com_equiv. intros σ.
-    apply com_eq_subrel_equiv.
-    apply loop_unroll_sound.
-Qed.
-
-Fixpoint iterate_opt (n:nat) (opt : com -> com) c :=
-  match n with
-  | 0 => c
-  | S n => iterate_opt n opt (opt c)
-  end.
-
-Lemma iterate_opt_sound :
-  forall n (opt : com -> com)  (OPTSOUND: forall c, c ≊ opt c) c,
-    c ≊ iterate_opt n opt c.
-Proof.
-  intros n opt OPTSOUND.
-  induction n; intros; simpl.
-  - reflexivity.
-  - rewrite <- IHn.
-    apply OPTSOUND.
-Qed.
-
-Definition optimize (n:nat) (c:com) : com :=
-  let c' := com_assocR (loop_unroll_com n c) in
-  iterate_opt n (fun c => fold_constants_com (propagate_com c)) c'.
-
-Lemma optimize_sound : forall n c,
-    c ≊ optimize n c.
-Proof.
-  intros n c.
-  unfold optimize.
-  rewrite <- iterate_opt_sound.
-  rewrite <- com_assocR_correct.
-  apply loop_unroll_com_sound.
-  intros c0.
-  rewrite fold_constants_com_sound.
-  apply propagate_com_sound.
-Qed.
-
-Opaque optimize_sound.
-
-(** Imp code for [factorial] for a specific number: *)
-Definition fact_n n := <{ X := n ; fact_in_coq }>.
-
-Definition fact_opt n :=
-  optimize (n+1) (fact_n n).
-
-Definition fact_opt8 := fact_opt 8.
-Eval compute in com_assocR fact_opt8.
-
-Definition fact_opt5 := fact_opt 5.
-
-Eval compute in fact_n 5.
-Eval compute in fact_opt5.
-
-Lemma fact_opt_correct : forall (n:nat),
-    <{ X := n ; fact_in_coq }> ≊ fact_opt n.
-Proof.
-  intros n.
-  unfold fact_in_coq.
-  apply optimize_sound.
-Qed.
-
-Lemma store_store_elimination_correct : forall x a1 a2,
-    (contains x a2 = false) ->
-    <{ x := a1 ; x := a2 }> ≊ <{ x := a2 }>.
-Proof.
-  intros x a1 a2 H σ.
-  simpl.
-  norm.
-  cbn.
-  apply eutt_Ret.
-  specialize (contains_false_equiv x a2 H) as EQ.
-  rewrite <- EQ.
-  rewrite t_update_shadow.
-  reflexivity.
-Qed.
-
-Lemma asgn_commutes : forall (x y:string) a1 a2,
-    (contains x a2 = false) ->
-    (contains y a1 = false) ->
-    x <> y ->
-    <{ x := a1 ; y := a2 }> ≊ <{ y := a2; x := a1 }>.
-Proof.
-  intros x y a1 a2 C1 C2 NEQ σ.
-  simpl.
-  norm.
-  cbn.
-  apply eutt_Ret.
-  simpl.
-  specialize (contains_false_equiv x a2 C1) as EQ1.
-  rewrite <- EQ1.
-  specialize (contains_false_equiv y a1 C2) as EQ2.
-  rewrite <- EQ2.
-  rewrite t_update_permute; auto.
-Qed.
-
-Eval compute in fact_opt5.
-
-(**
-
-x1 = a1 ; x2 = a2 ; x3 = a3 ; c
-x1 = x3
-x1 = a1 ; x2 = a2 ; x1 = a3 ; c   // x1 <> x2 /\ not (contains x1 a2)  /\ not (contains x2 a3)
-x1 = a1 ; x1 = a3 ; x2 = a2 ; c
-x1 = a3 ; x2 = a2 ; c             // not contains x1 a3
-*)
-
-Fixpoint dead_store_elimination (c:com) : com :=
-  match c with
-  | <{ skip }> => c
-  | <{ x := a }> => c
-  | <{ x1 := a1; c2 }> =>
-      let c2' := dead_store_elimination c2 in
-      match c2' with
-      | <{ x2 := a2 }> =>
-          if ((String.eqb x1 x2)
-              && negb (contains x1 a2))%bool
-          then
-            <{ x2 := a2 }>
-          else
-            <{ x1 := a1 ; c2' }>
-      | <{ x2 := a2 ; c3' }> =>
-          match c3' with
-          | <{ x3 := a3 }> =>
-              if (String.eqb x1 x3
-                  && negb (String.eqb x2 x3)
-                  && negb (contains x3 a2)
-                  && negb (contains x2 a3)
-                  && negb (contains x1 a3))%bool
-              then <{ x3 := a3 ; x2 := a2 }>
-              else <{ x1 := a1 ; c2' }>
-          | <{ x3 := a3 ; c4' }> =>
-              if (String.eqb x1 x3
-                  &&  negb (String.eqb x2 x3)
-                  && negb (contains x3 a2)
-                  && negb (contains x2 a3)
-                  && negb (contains x1 a3))%bool
-              then <{ x3 := a3 ; x2 := a2 ; c4' }>
-              else if ((String.eqb x1 x2)
-                       && negb (String.eqb x2 x3)
-                       && negb (contains x1 a2))%bool
-                   then <{ x2 := a2 ; x3 := a3 ; c4' }>
-                   else <{ x1 := a1 ; c2' }>
-          | _ =>
-              if ((String.eqb x1 x2)
-                  && negb (contains x1 a2))%bool
-              then
-                <{ x2 := a2 ; c3' }>
-              else
-                <{ x1 := a1 ; c2' }>
-          end
-      | _ => <{ x1 := a1 ; c2' }>
-      end
-  | <{ c1 ; c2 }> =>
-      let c2' := dead_store_elimination c2 in
-      <{ c1 ; c2' }>
-  | <{ if b then c1 else c2 end }> =>
-      let c1' := dead_store_elimination c1 in
-      let c2' := dead_store_elimination c2 in
-      <{ if  b then c1' else c2' end }>
-  | <{ while b do c end }> =>
-      let c' := dead_store_elimination c in
-      <{ while b do c' end }>
-  end.
-
-Eval compute in (dead_store_elimination <{ X := 0 ; Y := 1 ; Y := 2 ; skip }>).
-Eval compute in (dead_store_elimination (com_assocR fact_opt5)).
-Eval compute in (dead_store_elimination <{ Y := 120; Z := 0; skip }>).
-Eval compute in (dead_store_elimination <{ Y:= 0; Y := 120; Z := 0; skip }>).
-
-Lemma dead_store_elimination_correct :
-  forall c,
-    c ≊ (dead_store_elimination c).
-Proof.
-  induction c; simpl; try reflexivity.
-  - destruct c1; simpl; try (rewrite <- IHc2; try reflexivity).
-    + destruct (dead_store_elimination c2); simpl; try (rewrite <- IHc2; try reflexivity).
-      * destruct (String.eqb_spec x x0); subst; simpl.
-        2: { rewrite IHc2. reflexivity. }
-        destruct (contains x0 a0) eqn : HC; simpl.
-        1: { rewrite IHc2. reflexivity. }
-        rewrite IHc2. apply store_store_elimination_correct; auto.
-      * destruct c1; simpl; try (rewrite <- IHc2; try reflexivity).
-        destruct c3.
-        -- destruct (String.eqb_spec x x0); subst; simpl.
-           2:{ rewrite IHc2. reflexivity. }
-           destruct (contains x0 a0) eqn : HC; simpl.
-           rewrite IHc2. reflexivity.
-           rewrite IHc2. rewrite <- seqA_sound. rewrite store_store_elimination_correct; auto.
-           reflexivity.
-        -- destruct (String.eqb_spec x x1); subst; simpl.
-           2: { rewrite IHc2. reflexivity. }
-           destruct (String.eqb_spec x0 x1); subst; simpl.
-           1: { rewrite IHc2. reflexivity. }
-           destruct (contains x1 a0) eqn : HC1; simpl.
-           1: { rewrite IHc2. reflexivity. }
-           destruct (contains x0 a1) eqn : HC2; simpl.
-           1: { rewrite IHc2. reflexivity. }
-           destruct (contains x1 a1) eqn : HC3; simpl.
-           1: { rewrite IHc2. reflexivity. }
-           rewrite IHc2. rewrite asgn_commutes; auto.
-           rewrite <- seqA_sound.
-           rewrite store_store_elimination_correct; auto.
-           reflexivity.
-        -- destruct c3_1; simpl.
-           ** destruct (String.eqb_spec x x0); subst; simpl.
-              2 : { rewrite IHc2. reflexivity. }
-              destruct (contains x0 a0) eqn : HC1; simpl.
-              1 : { rewrite IHc2.  reflexivity. }
-              rewrite IHc2. rewrite <- seqA_sound.
-              rewrite store_store_elimination_correct; auto.
-              reflexivity.
-           ** destruct (String.eqb_spec x x1); subst; simpl.
-              1: { destruct (String.eqb_spec x0 x1); subst; simpl.
-                   destruct (String.eqb_spec x1 x1); subst; simpl.
-                   2: { contradiction. }
-                   rewrite IHc2. reflexivity.
-                   destruct (contains x1 a0) eqn : HC; simpl.
-                   destruct (String.eqb_spec x1 x0); subst; simpl.
-                   destruct (contains x0 a) eqn : HC1; simpl.
-                   contradiction.
-                   contradiction.
-                   rewrite <- IHc2. reflexivity.
-                   destruct (contains x0 a1) eqn : HC1; subst; simpl.
-                   destruct (String.eqb_spec x1 x0); subst.
-                   contradiction.
-                   simpl.
-                   rewrite <- IHc2. reflexivity.
-                   destruct (contains x1 a1) eqn : HC2; subst; simpl.
-                   destruct (String.eqb_spec x1 x0); subst; simpl.
-                   contradiction.
-                   rewrite IHc2. reflexivity.
-                   rewrite <- seqA_sound in IHc2.
-                   rewrite asgn_commutes in IHc2; auto.
-                   rewrite seqA_sound in IHc2.
-                   rewrite IHc2.
-                   rewrite <- seqA_sound.
-                   rewrite store_store_elimination_correct; auto.
-                   reflexivity. }
-              destruct (String.eqb_spec x x0); subst; simpl.
-              2: { rewrite <- IHc2. reflexivity. }
-              destruct (String.eqb_spec x0 x1); subst; simpl.
-              rewrite IHc2. reflexivity.
-              destruct (contains x0 a0) eqn : HC; simpl.
-              rewrite IHc2. reflexivity.
-              rewrite IHc2.
-              rewrite <- seqA_sound.
-              rewrite store_store_elimination_correct; auto.
-              reflexivity.
-           ** destruct (String.eqb_spec x x0); simpl; subst.
-              destruct (contains x0 a0) eqn : HC; simpl.
-              rewrite IHc2. reflexivity.
-              rewrite IHc2.
-              rewrite <- seqA_sound.
-              rewrite store_store_elimination_correct; auto.
-              reflexivity.
-              rewrite IHc2. reflexivity.
-           ** destruct (String.eqb_spec x x0); simpl; subst.
-              destruct (contains x0 a0) eqn : HC; simpl.
-              rewrite IHc2. reflexivity.
-              rewrite IHc2.
-              rewrite <- seqA_sound.
-              rewrite store_store_elimination_correct; auto.
-              reflexivity.
-              rewrite IHc2. reflexivity.
-           ** destruct (String.eqb_spec x x0); simpl; subst.
-              destruct (contains x0 a0) eqn : HC; simpl.
-              rewrite IHc2. reflexivity.
-              rewrite IHc2.
-              rewrite <- seqA_sound.
-              rewrite store_store_elimination_correct; auto.
-              reflexivity.
-              rewrite IHc2. reflexivity.
-        -- destruct (String.eqb_spec x x0); simpl; subst.
-           destruct (contains x0 a0) eqn : HC; simpl.
-           rewrite IHc2. reflexivity.
-           rewrite IHc2.
-           rewrite <- seqA_sound.
-           rewrite store_store_elimination_correct; auto.
-              reflexivity.
-              rewrite IHc2. reflexivity.
-        -- destruct (String.eqb_spec x x0); simpl; subst.
-           destruct (contains x0 a0) eqn : HC; simpl.
-           rewrite IHc2. reflexivity.
-           rewrite IHc2.
-           rewrite <- seqA_sound.
-           rewrite store_store_elimination_correct; auto.
-              reflexivity.
-              rewrite IHc2. reflexivity.
-  - rewrite <- IHc1, <- IHc2. reflexivity.
-  - rewrite <- IHc. reflexivity.
-Qed.
-
-
-
-
-
-
-
-
-
-
-(** Example: using verified optimizations to prove an
-equivalence between Imp programs. *)
-
-Example opt_fact_sound :
-  <{ X := 5;
-     Z := X;
-     Y := 1;
-     while Z <> 0 do
-        Y := Y * Z;
-        Z := Z - 1
-     end }>
-    ≊
-  <{ X := 5; Z := 0; Y := 120 }>.
-Proof.
-  rewrite (optimize_sound 6).
-  cbn.
-  rewrite dead_store_elimination_correct.
-  cbn.
-  rewrite skipR_sound.
-  reflexivity.
-Qed.
-
-(* 2024-06-10 19:33 *)
+(* 2024-06-13 11:26 *)
