ImpOpt.v
@@ -1,0 +1,999 @@
+From Paco Require Import paco.
+From Coq Require Import Nat String RelationClasses Morphisms Psatz FunctionalExtensionality.
+From RIP Require Import Maps Imp Utils ImpDenotation ImpEquiv Hoare.
+From ITree Require Import ITree ITreeFacts Events.State Events.StateFacts HeterogeneousRelations.
+Import ITreeNotations.
+
+Notation "t1 ≈[ R ] t2" := (eutt R t1 t2) (at level 20).
+
+#[local]
+Hint Rewrite aexp_pure_aeval bexp_pure_beval : opt.
+
+(* ================================================================= *)
+(** ** Example: Variable Renaming *)
+
+Definition swapped (X Y : string) (σ1 σ2 : mem) : Prop :=
+  (forall Z, Z <> X /\ Z <> Y -> σ1 Z = σ2 Z)
+  /\ (σ1 X = σ2 Y)
+  /\ (σ1 Y = σ2 X).
+
+Example com1 := <{ X := X + Y; Z := X - Y }>.
+Example com2 := <{ Y := Y + X; Z := Y - X }>.
+
+Lemma swapped_correct :
+  forall σ1 σ2,
+    swapped X Y σ1 σ2 ->
+    (ℑ ⟦com1⟧ σ1)
+      ≈[ (prod_rel (swapped X Y) eq) ]
+    (ℑ ⟦com2⟧ σ2).
+Proof.
+  intros.
+  unfold com1, com2.
+  cbn.
+  norm.
+  apply eutt_Ret.
+  apply prod_morphism; cbn; auto.
+  unfold swapped.
+  destruct H as (H1 & H2 & H3).
+  unfold t_update.
+  split.
+  - intros Z [HX HY].
+    destruct (Imp.Z =? Z)%string.
+    rewrite H2. rewrite <- H3. reflexivity.
+    destruct (eqb_spec X Z).
+    subst. contradiction.
+    destruct (eqb_spec Y Z).
+    subst. contradiction.
+    apply H1. tauto.
+  - destruct (eqb_spec Z X). inversion e.
+    destruct (eqb_spec Z Y). inversion e.
+    destruct (eqb_spec X X).
+    destruct (eqb_spec Y Y).
+    destruct (eqb_spec X Y).
+    destruct (eqb_spec Y X).
+    rewrite H2; rewrite <- H3; auto.
+    inversion e1.
+    destruct (eqb_spec Y X).
+    inversion e1.
+    rewrite H2; rewrite <- H3; auto.
+    contradiction.
+    contradiction.
+Qed.
+
+
+(* ================================================================= *)
+(** ** Substitution *)
+
+(**
+  Substitutes an arbitary arithemetic expression for the variable [x] in
+*)
+Fixpoint substitute_aexp (x:string) (ax:aexp) (a:aexp) : aexp :=
+  match a with
+  | ANum n => a
+  | AId y => if String.eqb y x then ax else a
+  | <{ a1 + a2 }> =>
+      <{ (substitute_aexp x ax a1) + (substitute_aexp x ax a2) }>
+
+  | <{ a1 - a2 }> =>
+      <{ (substitute_aexp x ax a1) - (substitute_aexp x ax a2) }>
+
+  | <{ a1 * a2 }> =>
+      <{ (substitute_aexp x ax a1) * (substitute_aexp x ax a2) }>
+  end.
+
+Eval compute in (substitute_aexp X (<{ Y + 2}>) (<{ X + Z }>)).
+(** ==> [<{ Y + 2 + Z }>] *)
+
+(* TODO: Move this to ImpEquiv *)
+Lemma aexp_eval_semantics2 : forall a1 a2 σ,
+    (aeval σ a1 = aeval σ a2) <->
+      ℑ ⟦ a1 ⟧a σ ≈ ℑ ⟦ a2 ⟧a σ.
+Proof.
+  intros.
+  split.
+  - intros H.
+    norm.
+    rewrite H.
+    reflexivity.
+  - intros H.
+    unfold aexp_equiv in H.
+    do 2 rewrite aexp_pure_aeval in H.
+    apply eutt_Ret in H.
+    inversion H.
+    reflexivity.
+Qed.
+
+Lemma substitute_aexp_aeval : forall (x:string) ax a,
+  forall σ (EQ : aeval σ <{ x }> = aeval σ ax),
+    aeval σ a = aeval σ (substitute_aexp x ax a).
+Proof.
+  intros x ax a σ EQ.
+  induction a; simpl; auto.
+  destruct (String.eqb_spec x0 x).
+  - simpl in EQ. subst. assumption.
+  - reflexivity.
+Qed.
+
+(* ----------------------------------------------------------------- *)
+(** *** Correctness lemma *)
+
+Lemma substitute_aexp_semantic : forall (x:string) ax a,
+  forall σ (EQ: ℑ ⟦ <{ x }> ⟧a σ ≈ ℑ ⟦ ax ⟧a σ),
+    ℑ ⟦ a ⟧a σ
+      ≈
+    ℑ ⟦ substitute_aexp x ax a ⟧a σ.
+Proof.
+  intros x ax a σ HEQ.
+  apply aexp_eval_semantics2.
+  intros. apply substitute_aexp_aeval.
+  apply aexp_eval_semantics2.
+  assumption.
+Qed.
+
+(* TODO: Move to ImpEquiv.v *)
+Lemma bexp_eval_semantics : forall b1 b2 σ,
+    (beval σ b1 = beval σ b2) <->
+      ℑ ⟦ b1 ⟧b σ ≈ ℑ ⟦ b2 ⟧b σ.
+Proof.
+  intros.
+  split.
+  - intros H.
+    norm.
+    rewrite H.
+    reflexivity.
+  - intros H.
+    unfold bexp_equiv in H.
+    do 2 rewrite bexp_pure_beval in H.
+    apply eutt_Ret in H.
+    inversion H.
+    reflexivity.
+Qed.
+
+Fixpoint substitute_bexp (x:string) (ax:aexp) (b:bexp) : bexp :=
+  match b with
+  | <{true}>      => b
+  | <{false}>     => b
+  | <{a1 = a2}>   => <{ (substitute_aexp x ax a1) = (substitute_aexp x ax a2) }>
+  | <{a1 <> a2}>   => <{ (substitute_aexp x ax a1) <> (substitute_aexp x ax a2) }>
+  | <{a1 <= a2}>  => <{ (substitute_aexp x ax a1) <= (substitute_aexp x ax a2) }>
+  | <{a1 > a2}>   => <{ (substitute_aexp x ax a1) > (substitute_aexp x ax a2) }>
+  | <{~ b1}>      => <{~ (substitute_bexp x ax b1) }>
+  | <{b1 && b2}>  => <{ (substitute_bexp x ax b1) && (substitute_bexp x ax b2) }>
+  end.
+
+Lemma substitute_bexp_beval : forall (x:string) ax b,
+  forall σ (EQ : aeval σ <{ x }> = aeval σ ax),
+    beval σ b = beval σ (substitute_bexp x ax b).
+Proof.
+  intros x ax b σ EQ.
+  induction b; simpl; try reflexivity.
+  - repeat rewrite <- (substitute_aexp_aeval x ax); auto.
+  - repeat rewrite <- (substitute_aexp_aeval x ax); auto.
+  - repeat rewrite <- (substitute_aexp_aeval x ax); auto.
+  - repeat rewrite <- (substitute_aexp_aeval x ax); auto.
+  - rewrite IHb. reflexivity.
+  - rewrite IHb1, IHb2. reflexivity.
+Qed.
+
+Lemma substitute_bexp_semantic : forall (x:string) ax b,
+  forall σ (EQ: ℑ ⟦ <{ x }> ⟧a σ ≈ ℑ ⟦ ax ⟧a σ),
+    ℑ ⟦ b ⟧b σ ≈ ℑ ⟦ substitute_bexp x ax b ⟧b σ.
+Proof.
+  intros x ax a σ HEQ.
+  apply bexp_eval_semantics.
+  intros. apply substitute_bexp_beval.
+  apply aexp_eval_semantics2.
+  assumption.
+Qed.
+
+Fixpoint contains (x:string) (a:aexp) : bool :=
+  match a with
+  | ANum n => false
+  | AId y => String.eqb y x
+  | <{ a1 + a2 }> => (contains x a1 || contains x a2)%bool
+  | <{ a1 - a2 }> => (contains x a1 || contains x a2)%bool
+  | <{ a1 * a2 }> => (contains x a1 || contains x a2)%bool
+  end.
+
+Lemma contains_false_equiv: forall (y:string) a,
+    contains y a = false ->
+    forall (σ:state) n, aeval σ a = aeval ( y !-> n ; σ ) a.
+Proof.
+  intros y.
+  induction a; intros HC σ m; simpl in *; try reflexivity.
+  - destruct (String.eqb_spec x y).
+    + inversion HC.
+    + rewrite t_update_neq; auto.
+  - apply Bool.orb_false_elim in HC.
+    destruct HC as [HA1 HA2].
+    auto.
+  - apply Bool.orb_false_elim in HC.
+    destruct HC as [HA1 HA2].
+    auto.
+  - apply Bool.orb_false_elim in HC.
+    destruct HC as [HA1 HA2].
+    auto.
+Qed.
+
+(* ----------------------------------------------------------------- *)
+(** *** Substitution in a command *)
+
+(** Because commands are not pure, we can't blindly substitute. *)
+
+Fixpoint substitute_com (x:string) (ax:aexp) (c:com) : (com * bool) :=
+  match c with
+  | <{ skip }> => (c, false)
+  | <{ y := a }> =>
+      let a' := substitute_aexp x ax a in
+      (<{ y := a' }>, ((y =? x)%string || contains y ax)%bool)
+  | <{ c1 ; c2 }> =>
+      let '(c1', stop1) := substitute_com x ax c1 in
+      if stop1
+      then (<{ c1' ; c2 }>, stop1)
+      else
+        let '(c2', stop2) := substitute_com x ax c2 in
+        (<{ c1' ; c2' }>, stop2)
+  | <{ if b then c1 else c2 end }> =>
+      let '(c1', stop1) := substitute_com x ax c1 in
+      let '(c2', stop2) := substitute_com x ax c2 in
+      (<{ if (substitute_bexp x ax b) then c1' else c2' end }>, (stop1 || stop2)%bool)
+  | <{ while b do c end }> =>
+      let '(c', stop) := substitute_com x ax c in
+      if stop then (<{ while b do c end }>, true)
+      else (<{ while (substitute_bexp x ax b) do c' end}>, false)
+  end.
+
+(** Examples of when it is OK (or not) to substitute: *)
+Eval compute in substitute_com X 0 <{ Z := 3; Y := X + X ; Y := X }>.
+Eval compute in substitute_com X 0 <{ X := 3; X := X + X ; Y := X }>.
+
+(* ----------------------------------------------------------------- *)
+(** *** Correctness of substition *)
+
+(** Define an invariant that says when we can safely substitute the
+expression  <{ ax }> for <{ x }> in a state σ.  *)
+
+Definition subst_invariant x ax σ :=
+  aeval σ <{ x }> = aeval σ ax.
+
+(** Define the relational post condition for reasoning about the
+results of substitution, relative to the initial state [σ]. *)
+
+Definition post_condition x ax b (σ0:state) :=
+  fun σ1 σ2 =>
+    σ1 = σ2
+    /\ (* If the substitution claims [x] and [ax] were _not_ modified... *)
+      (b = false ->
+       (σ1 x = σ0 x (* ...then [x] wasn't modified *)
+        /\ (* ... and neither was [ax]  *)
+          aeval σ0 ax = aeval σ1 ax
+          (* ... and the invariant preserved *)
+        /\ subst_invariant x ax σ1)).
+
+(* ----------------------------------------------------------------- *)
+(** *** Some properties of the predicates *)
+#[local]
+ Instance post_condition_refl : forall x ax σ,
+    Reflexive (post_condition x ax true σ).
+Proof.
+  intros.
+  red.
+  intros.
+  unfold post_condition.
+  split. reflexivity. intros. inversion H.
+Qed.
+
+Lemma post_condition_mono : forall x ax σ st1 st2 b1 b2,
+    (b1 = true -> b2 = true) ->
+    post_condition x ax b1 σ st1 st2 ->
+    post_condition x ax b2 σ st1 st2.
+Proof.
+  intros.
+  unfold post_condition in *.
+  intuition.
+  - destruct b1.
+    + rewrite H in H0. inversion H0. reflexivity.
+    + apply H2. reflexivity.
+  - destruct b1.
+    + rewrite H in H0. inversion H0. reflexivity.
+    + apply H2. reflexivity.
+  - unfold subst_invariant in *. destruct b1.
+    + intuition. subst.  inversion H3.
+    + intuition.
+Qed.
+
+(* ----------------------------------------------------------------- *)
+(** *** A relational specification *)
+Lemma substitute_com_correct :
+  forall x ax c c' b
+    (HS: substitute_com x ax c = (c', b)),
+  forall σ (P: subst_invariant x ax σ),
+      (ℑ ⟦c⟧ σ)
+        ≈[ (prod_rel (post_condition x ax b σ) eq)]
+      (ℑ ⟦c'⟧ σ).
+(* TODO: Clean up this proof! *)
+Proof.
+  intros x ax c.
+  induction c; intros; simpl in HS; inversion HS; subst; simpl; norm.
+  - apply eutt_Ret. unfold post_condition. auto.
+  - apply eutt_Ret.
+    simpl.
+    constructor; auto.
+    split; simpl; auto.
+    + rewrite <- substitute_aexp_aeval; auto.
+    + intros H.
+      destruct (String.eqb_spec x0 x).
+      * subst. simpl in H. inversion H.
+      * repeat split.
+       -- rewrite Bool.orb_false_l in H.
+          unfold subst_invariant in P.
+          apply t_update_neq.
+          assumption.
+       -- simpl in H.
+          erewrite contains_false_equiv. reflexivity.
+          assumption.
+       -- rewrite Bool.orb_false_l in H.
+          unfold subst_invariant in *.
+          erewrite <- contains_false_equiv.
+          erewrite <- contains_false_equiv; assumption.
+          cbn. apply eqb_neq. auto.
+  - destruct (substitute_com x ax c1).
+    specialize (IHc1 c b0 eq_refl σ P).
+    destruct b0.
+    + inversion HS. subst.
+      cbn.
+      norm.
+      eapply eutt_clo_bind.
+      apply IHc1.
+      intros u1 u2 HP.
+      destruct u1, u2, u, u0.
+      cbn.
+      destruct HP as [HM _].
+      destruct HM. simpl in H.
+      subst.
+      reflexivity.
+    + destruct (substitute_com x ax c2).
+      inversion HS. subst.
+      cbn.
+      norm.
+      eapply eutt_clo_bind.
+      apply IHc1.
+      intros u1 u2 HP.
+      destruct u1, u2, u, u0.
+      cbn.
+      destruct HP as [[HM H]].
+      simpl in HM.
+      subst.
+      specialize (H eq_refl).
+      destruct H as [HM HE].
+      simpl in *.
+      destruct HE as [HE H].
+      specialize (IHc2 c0 b eq_refl m0 H).
+      eapply eutt_subrel.
+      2: { apply IHc2. }
+      intros. unfold post_condition in H1.
+      inversion H1.
+      destruct a, u, b0, u.
+      constructor; auto.
+      unfold post_condition.
+      intuition.
+  - destruct (substitute_com x ax c1).
+    destruct (substitute_com x ax c2).
+    cbn.
+    inversion HS. subst.
+    cbn.
+    norm.
+    cbn.
+    rewrite <- substitute_bexp_beval; auto.
+    destruct (beval σ b).
+    + eapply eutt_subrel.
+      2:{ apply IHc1; auto. }
+      intros. constructor.
+      eapply post_condition_mono.
+      2: { apply H. }
+      intros. intuition.
+      inversion H; auto.
+    + eapply eutt_subrel.
+      2: { apply IHc2; auto. }
+      intros.
+      constructor.
+      eapply post_condition_mono.
+      2: { apply H. }
+      intros. intuition.
+      inversion H; auto.
+  - destruct (substitute_com x ax c).
+    destruct b1.
+    + inversion HS. subst.
+      reflexivity.
+    + inversion HS.
+      subst. clear HS H0.
+      cbn.
+      specialize (IHc c0 false eq_refl).
+      eapply eutt_subrel.
+      2 : { eapply eutt_interp_state_iter with (RS := post_condition x ax false σ)(RA := eq)(RB := eq).
+            intros.
+            unfold subst_invariant in *.
+            intuition. subst.
+            norm. cbn.
+            rewrite <- substitute_bexp_beval.
+            unfold post_condition in H.
+            intuition.  subst.
+            unfold subst_invariant in H3.
+            destruct (beval s2 b).
+            norm.
+            eapply eutt_clo_bind.
+            apply IHc. assumption.
+            intros. norm.  destruct u1. destruct u2.
+           apply eutt_Ret. cbn. apply prod_morphism. simpl.
+           apply fst_rel in H0. simpl in H0. unfold post_condition in H0. intuition.
+           subst.
+           unfold post_condition.
+           split; auto.
+           intros. intuition.
+           eapply snd_rel in H0. cbn. cbn in H0. subst. econstructor. reflexivity.
+           norm. apply eutt_Ret. apply prod_morphism. simpl.
+           unfold post_condition.
+           split; auto. cbn.  constructor. reflexivity.
+           unfold post_condition in H.
+           intuition.  subst. unfold subst_invariant in H3. subst.
+           intuition.
+           unfold subst_invariant in *.
+           unfold post_condition.
+           split; auto.
+           reflexivity. }
+      intros.
+      destruct a, b0.
+      cbn in *.
+      apply prod_morphism.
+      cbn.  intuition.  cbn. intuition.
+Qed.
+
+Lemma subst_invariant_good : forall (x:string) a σ,
+    contains x a = false ->
+    subst_invariant x a (x !-> aeval σ a; σ).
+Proof.
+  intros.
+  unfold subst_invariant.
+  eapply contains_false_equiv in H.
+  rewrite <- H.
+  symmetry.
+  simpl.
+  rewrite t_update_eq.
+  reflexivity.
+Qed.
+
+(** *)
+Lemma substitute_com_subst : forall c x a σ,
+    contains x a = false ->
+    ℑ ⟦ c ⟧ (x !-> aeval σ a; σ)
+      ≈
+    ℑ ⟦ fst (substitute_com x a c) ⟧ (x !-> aeval σ a; σ).
+Proof.
+  intros.
+  destruct (substitute_com x a c) eqn:HS.
+  simpl.
+  apply substitute_com_correct with (σ := (x !-> aeval σ a; σ)) in HS.
+  eapply eutt_subrel.
+  2: { apply HS. }
+  intros.
+  destruct a0, u, b0, u.
+  inversion H0; clear H0.
+  unfold post_condition in fst_rel.
+  simpl in *.
+  intuition. subst. tauto.
+  apply subst_invariant_good.
+  assumption.
+Qed.
+
+Fixpoint com_append (c1 c2 : com) : com :=
+  match c1 with
+  | <{ skip }> => c2
+  | <{ c11 ; c12}> => <{ c11 ; (com_append c12 c2) }>
+  | _ => <{ c1 ; c2 }>
+  end.
+
+Lemma com_append_correct : forall c1 c2,
+    com_append c1 c2 ≡ <{ c1 ; c2 }>.
+Proof.
+  induction c1; intro c2; simpl; try reflexivity.
+  - rewrite skipL_sound. reflexivity.
+  - rewrite seqA_sound. rewrite IHc1_2. reflexivity.
+Qed.
+
+#[global]
+ Instance Proper_com_append: Proper (com_eq ==> com_eq ==> com_eq) com_append.
+Proof.
+  intros c11.
+  destruct c11; intros c12 EQ1 c21 c22 EQ2; simpl.
+  - rewrite com_append_correct. rewrite <- EQ1. rewrite skipL_sound. assumption.
+  - rewrite EQ1. rewrite com_append_correct. rewrite EQ2. reflexivity.
+  - rewrite com_append_correct. rewrite com_append_correct. rewrite <- EQ1.
+    rewrite seqA_sound. rewrite EQ2. reflexivity.
+  - rewrite com_append_correct. rewrite <- EQ1. rewrite EQ2. reflexivity.
+  - rewrite com_append_correct. rewrite <- EQ1. rewrite EQ2. reflexivity.
+Qed.
+
+Fixpoint com_assocR c : com :=
+  match c with
+  | <{ skip }> => c
+  | <{ y := a }> => c
+  | <{ c1 ; c2 }> =>
+      let c1' := com_assocR c1 in
+      let c2' := com_assocR c2 in
+      com_append c1' c2'
+  | <{ if b then c1 else c2 end }> =>
+      let c1' := com_assocR c1 in
+      let c2' := com_assocR c2 in
+      <{ if b then c1' else c2' end }>
+  | <{ while b do c end }> =>
+      let c' := com_assocR c in
+      <{ while b do c' end }>
+  end.
+
+Lemma com_assocR_correct : forall c,
+    c ≡ com_assocR c.
+Proof.
+  induction c; simpl; try reflexivity.
+  - rewrite <- IHc1. rewrite <- IHc2.
+    rewrite com_append_correct.
+    reflexivity.
+  - rewrite <- IHc1. rewrite <- IHc2.
+    reflexivity.
+  - rewrite <- IHc. reflexivity.
+Qed.
+
+(* ----------------------------------------------------------------- *)
+(** *** Constant propagation as a function on syntax *)
+
+Fixpoint propagate_com (c:com) : com :=
+  match c with
+  | <{ skip }> => c
+  | <{ y := a }> => c
+  | <{ y := a ; c2 }> =>
+      let c2' := propagate_com c2 in
+      if contains y a
+      then <{ y := a ; c2' }>
+      else <{ y := a;  fst (substitute_com y a c2') }>
+  | <{ c1 ; c2 }> =>
+      let c1' := propagate_com c1 in
+      let c2' := propagate_com c2 in
+      <{ c1' ; c2' }>
+  | <{ if b then c1 else c2 end }> =>
+      let c1' := propagate_com c1 in
+      let c2' := propagate_com c2 in
+      <{ if  b then c1' else c2' end }>
+  | <{ while b do c end }> =>
+      let c' := propagate_com c in
+      <{ while b do c' end }>
+  end.
+
+
+Lemma propagate_com_sound : forall c,
+    c ≊ (propagate_com c).
+Proof.
+  induction c.
+  - simpl. reflexivity.
+  - simpl. reflexivity.
+  - simpl.
+    destruct c1.
+    + simpl. rewrite <- IHc2. reflexivity.
+    + destruct (contains x a) eqn:H.
+      * rewrite <- IHc2. reflexivity.
+      * intro.
+        cbn.
+        norm.
+        cbn.
+        eapply transitivity.
+        apply IHc2.
+        apply substitute_com_subst.
+        assumption.
+    + rewrite <- IHc1. rewrite <- IHc2. reflexivity.
+    + simpl in *.
+      rewrite IHc1.
+      rewrite <- IHc2.
+      reflexivity.
+    + simpl. rewrite <- IHc1. rewrite <- IHc2. reflexivity.
+  - simpl. rewrite <- IHc1. rewrite <- IHc2. reflexivity.
+  - simpl. rewrite <- IHc. reflexivity.
+Qed.
+
+(* ----------------------------------------------------------------- *)
+(** *** An Exmple *)
+
+Definition example : com :=
+  <{ X := 4 + 5;
+     Y := X;
+     if ((X - Y) = (2 + 4)) then skip
+     else Y := X end;
+     if (0 <= (4 - (2 + 1))) then Y := 0
+     else skip end;
+     while (Y = 0) do
+             X := X + 1
+             end
+    }>.
+
+Eval compute in fold_constants_com (propagate_com example).
+(** ==>
+
+<{ X := 9; Y := 9; Y := 9; Y := 0; while Y = 0 do X := X + 1 end }>.
+Proof.
+*)
+
+Example correct: example ≊ (fold_constants_com (propagate_com example)).
+Proof.
+  rewrite fold_constants_com_sound.
+  apply propagate_com_sound.
+Qed.
+
+(* ----------------------------------------------------------------- *)
+(** *** Loop unrolling *)
+
+Fixpoint loop_unroll_while (n:nat) (b:bexp) (c:com) : com :=
+  match n with
+  | 0 => <{ while b do c end }>
+  | S n => <{ if b then c ; (loop_unroll_while n b c) else skip end }>
+  end.
+
+Lemma loop_unroll_sound : forall (n:nat) (b:bexp) (c:com),
+    <{ while b do c end }> ≡ loop_unroll_while n b c.
+Proof.
+  induction n; intros; simpl.
+  - reflexivity.
+  - rewrite <- IHn.
+    apply loop_unroll1_sound_strong.
+Qed.
+
+Fixpoint loop_unroll_com n (c:com) : com :=
+  match c with
+  | <{ skip }> => c
+  | <{ y := a }> => c
+  | <{ c1 ; c2 }> =>
+      let c1' := loop_unroll_com n c1 in
+      let c2' := loop_unroll_com n c2 in
+      <{ c1' ; c2' }>
+  | <{ if b then c1 else c2 end }> =>
+      let c1' := loop_unroll_com n c1 in
+      let c2' := loop_unroll_com n c2 in
+      <{ if  b then c1' else c2' end }>
+  | <{ while b do c end }> =>
+      loop_unroll_while n b c
+  end.
+
+Lemma loop_unroll_com_sound : forall n c,
+    c ≊ (loop_unroll_com n c).
+Proof.
+  induction c.
+  - simpl. reflexivity.
+  - simpl. reflexivity.
+  - simpl. rewrite <- IHc1. rewrite <- IHc2. reflexivity.
+  - simpl. rewrite <- IHc1. rewrite <- IHc2. reflexivity.
+  - simpl. unfold com_equiv. intros σ.
+    apply com_eq_subrel_equiv.
+    apply loop_unroll_sound.
+Qed.
+
+(* ----------------------------------------------------------------- *)
+(** *** Run several passes of an optimization function *)
+
+Fixpoint iterate_opt (n:nat) (opt : com -> com) c :=
+  match n with
+  | 0 => c
+  | S n => iterate_opt n opt (opt c)
+  end.
+
+Lemma iterate_opt_sound :
+  forall n (opt : com -> com)  (OPTSOUND: forall c, c ≊ opt c) c,
+    c ≊ iterate_opt n opt c.
+Proof.
+  intros n opt OPTSOUND.
+  induction n; intros; simpl.
+  - reflexivity.
+  - rewrite <- IHn.
+    apply OPTSOUND.
+Qed.
+
+(* ----------------------------------------------------------------- *)
+(** *** An Imp optimization pass *)
+
+Definition optimize (n:nat) (c:com) : com :=
+  let c' := com_assocR (loop_unroll_com n c) in
+  iterate_opt n (fun c => fold_constants_com (propagate_com c)) c'.
+
+Lemma optimize_sound : forall n c,
+    c ≊ optimize n c.
+Proof.
+  intros n c.
+  unfold optimize.
+  rewrite <- iterate_opt_sound.
+  rewrite <- com_assocR_correct.
+  apply loop_unroll_com_sound.
+  intros c0.
+  rewrite fold_constants_com_sound.
+  apply propagate_com_sound.
+Qed.
+
+(* ----------------------------------------------------------------- *)
+(** *** Back to our factorial example
+
+    Imp code for [factorial] for a specific number: *)
+Definition fact_n n := <{ X := n ; fact_in_coq }>.
+
+Definition fact_opt n :=
+  optimize (n+1) (fact_n n).
+
+Definition fact_opt5 := fact_opt 5.
+
+Lemma fact_opt_correct : forall (n:nat),
+    <{ X := n ; fact_in_coq }> ≊ fact_opt n.
+Proof.
+  intros n.
+  unfold fact_in_coq.
+  apply optimize_sound.
+Qed.
+
+(* ----------------------------------------------------------------- *)
+(** *** Dead store elimination *)
+
+(** We'll skip the full story, but see how we can justify: *)
+
+Lemma store_store_elimination_correct : forall x a1 a2,
+    (contains x a2 = false) ->
+    <{ x := a1 ; x := a2 }> ≊ <{ x := a2 }>.
+Proof.
+  intros x a1 a2 H σ.
+  simpl.
+  norm.
+  cbn.
+  apply eutt_Ret.
+  specialize (contains_false_equiv x a2 H) as EQ.
+  rewrite <- EQ.
+  rewrite t_update_shadow.
+  reflexivity.
+Qed.
+
+Lemma asgn_commutes : forall (x y:string) a1 a2,
+    (contains x a2 = false) ->
+    (contains y a1 = false) ->
+    x <> y ->
+    <{ x := a1 ; y := a2 }> ≊ <{ y := a2; x := a1 }>.
+Proof.
+  intros x y a1 a2 C1 C2 NEQ σ.
+  simpl.
+  norm.
+  cbn.
+  apply eutt_Ret.
+  simpl.
+  specialize (contains_false_equiv x a2 C1) as EQ1.
+  rewrite <- EQ1.
+  specialize (contains_false_equiv y a1 C2) as EQ2.
+  rewrite <- EQ2.
+  rewrite t_update_permute; auto.
+Qed.
+
+(**
+
+x1 = a1 ; x2 = a2 ; x3 = a3 ; c
+x1 = x3
+x1 = a1 ; x2 = a2 ; x1 = a3 ; c   // x1 <> x2 /\ not (contains x1 a2)  /\ not (contains x2 a3)
+x1 = a1 ; x1 = a3 ; x2 = a2 ; c
+x1 = a3 ; x2 = a2 ; c             // not contains x1 a3
+*)
+
+Fixpoint dead_store_elimination (c:com) : com :=
+  match c with
+  | <{ skip }> => c
+  | <{ x := a }> => c
+  | <{ x1 := a1; c2 }> =>
+      let c2' := dead_store_elimination c2 in
+      match c2' with
+      | <{ x2 := a2 }> =>
+          if ((String.eqb x1 x2)
+              && negb (contains x1 a2))%bool
+          then
+            <{ x2 := a2 }>
+          else
+            <{ x1 := a1 ; c2' }>
+      | <{ x2 := a2 ; c3' }> =>
+          match c3' with
+          | <{ x3 := a3 }> =>
+              if (String.eqb x1 x3
+                  && negb (String.eqb x2 x3)
+                  && negb (contains x3 a2)
+                  && negb (contains x2 a3)
+                  && negb (contains x1 a3))%bool
+              then <{ x3 := a3 ; x2 := a2 }>
+              else <{ x1 := a1 ; c2' }>
+          | <{ x3 := a3 ; c4' }> =>
+              if (String.eqb x1 x3
+                  &&  negb (String.eqb x2 x3)
+                  && negb (contains x3 a2)
+                  && negb (contains x2 a3)
+                  && negb (contains x1 a3))%bool
+              then <{ x3 := a3 ; x2 := a2 ; c4' }>
+              else if ((String.eqb x1 x2)
+                       && negb (String.eqb x2 x3)
+                       && negb (contains x1 a2))%bool
+                   then <{ x2 := a2 ; x3 := a3 ; c4' }>
+                   else <{ x1 := a1 ; c2' }>
+          | _ =>
+              if ((String.eqb x1 x2)
+                  && negb (contains x1 a2))%bool
+              then
+                <{ x2 := a2 ; c3' }>
+              else
+                <{ x1 := a1 ; c2' }>
+          end
+      | _ => <{ x1 := a1 ; c2' }>
+      end
+  | <{ c1 ; c2 }> =>
+      let c2' := dead_store_elimination c2 in
+      <{ c1 ; c2' }>
+  | <{ if b then c1 else c2 end }> =>
+      let c1' := dead_store_elimination c1 in
+      let c2' := dead_store_elimination c2 in
+      <{ if  b then c1' else c2' end }>
+  | <{ while b do c end }> =>
+      let c' := dead_store_elimination c in
+      <{ while b do c' end }>
+  end.
+
+Eval compute in (dead_store_elimination <{ X := 0 ; Y := 1 ; Y := 2 ; skip }>).
+Eval compute in (dead_store_elimination (com_assocR fact_opt5)).
+Eval compute in (dead_store_elimination <{ Y := 120; Z := 0; skip }>).
+Eval compute in (dead_store_elimination <{ Y:= 0; Y := 120; Z := 0; skip }>).
+
+Lemma dead_store_elimination_correct :
+  forall c,
+    c ≊ (dead_store_elimination c).
+Proof.
+  induction c; simpl; try reflexivity.
+  - destruct c1; simpl; try (rewrite <- IHc2; try reflexivity).
+    + destruct (dead_store_elimination c2); simpl; try (rewrite <- IHc2; try reflexivity).
+      * destruct (String.eqb_spec x x0); subst; simpl.
+        2: { rewrite IHc2. reflexivity. }
+        destruct (contains x0 a0) eqn : HC; simpl.
+        1: { rewrite IHc2. reflexivity. }
+        rewrite IHc2. apply store_store_elimination_correct; auto.
+      * destruct c1; simpl; try (rewrite <- IHc2; try reflexivity).
+        destruct c3.
+        -- destruct (String.eqb_spec x x0); subst; simpl.
+           2:{ rewrite IHc2. reflexivity. }
+           destruct (contains x0 a0) eqn : HC; simpl.
+           rewrite IHc2. reflexivity.
+           rewrite IHc2. rewrite <- seqA_sound. rewrite store_store_elimination_correct; auto.
+           reflexivity.
+        -- destruct (String.eqb_spec x x1); subst; simpl.
+           2: { rewrite IHc2. reflexivity. }
+           destruct (String.eqb_spec x0 x1); subst; simpl.
+           1: { rewrite IHc2. reflexivity. }
+           destruct (contains x1 a0) eqn : HC1; simpl.
+           1: { rewrite IHc2. reflexivity. }
+           destruct (contains x0 a1) eqn : HC2; simpl.
+           1: { rewrite IHc2. reflexivity. }
+           destruct (contains x1 a1) eqn : HC3; simpl.
+           1: { rewrite IHc2. reflexivity. }
+           rewrite IHc2. rewrite asgn_commutes; auto.
+           rewrite <- seqA_sound.
+           rewrite store_store_elimination_correct; auto.
+           reflexivity.
+        -- destruct c3_1; simpl.
+           ** destruct (String.eqb_spec x x0); subst; simpl.
+              2 : { rewrite IHc2. reflexivity. }
+              destruct (contains x0 a0) eqn : HC1; simpl.
+              1 : { rewrite IHc2.  reflexivity. }
+              rewrite IHc2. rewrite <- seqA_sound.
+              rewrite store_store_elimination_correct; auto.
+              reflexivity.
+           ** destruct (String.eqb_spec x x1); subst; simpl.
+              1: { destruct (String.eqb_spec x0 x1); subst; simpl.
+                   destruct (String.eqb_spec x1 x1); subst; simpl.
+                   2: { contradiction. }
+                   rewrite IHc2. reflexivity.
+                   destruct (contains x1 a0) eqn : HC; simpl.
+                   destruct (String.eqb_spec x1 x0); subst; simpl.
+                   destruct (contains x0 a) eqn : HC1; simpl.
+                   contradiction.
+                   contradiction.
+                   rewrite <- IHc2. reflexivity.
+                   destruct (contains x0 a1) eqn : HC1; subst; simpl.
+                   destruct (String.eqb_spec x1 x0); subst.
+                   contradiction.
+                   simpl.
+                   rewrite <- IHc2. reflexivity.
+                   destruct (contains x1 a1) eqn : HC2; subst; simpl.
+                   destruct (String.eqb_spec x1 x0); subst; simpl.
+                   contradiction.
+                   rewrite IHc2. reflexivity.
+                   rewrite <- seqA_sound in IHc2.
+                   rewrite asgn_commutes in IHc2; auto.
+                   rewrite seqA_sound in IHc2.
+                   rewrite IHc2.
+                   rewrite <- seqA_sound.
+                   rewrite store_store_elimination_correct; auto.
+                   reflexivity. }
+              destruct (String.eqb_spec x x0); subst; simpl.
+              2: { rewrite <- IHc2. reflexivity. }
+              destruct (String.eqb_spec x0 x1); subst; simpl.
+              rewrite IHc2. reflexivity.
+              destruct (contains x0 a0) eqn : HC; simpl.
+              rewrite IHc2. reflexivity.
+              rewrite IHc2.
+              rewrite <- seqA_sound.
+              rewrite store_store_elimination_correct; auto.
+              reflexivity.
+           ** destruct (String.eqb_spec x x0); simpl; subst.
+              destruct (contains x0 a0) eqn : HC; simpl.
+              rewrite IHc2. reflexivity.
+              rewrite IHc2.
+              rewrite <- seqA_sound.
+              rewrite store_store_elimination_correct; auto.
+              reflexivity.
+              rewrite IHc2. reflexivity.
+           ** destruct (String.eqb_spec x x0); simpl; subst.
+              destruct (contains x0 a0) eqn : HC; simpl.
+              rewrite IHc2. reflexivity.
+              rewrite IHc2.
+              rewrite <- seqA_sound.
+              rewrite store_store_elimination_correct; auto.
+              reflexivity.
+              rewrite IHc2. reflexivity.
+           ** destruct (String.eqb_spec x x0); simpl; subst.
+              destruct (contains x0 a0) eqn : HC; simpl.
+              rewrite IHc2. reflexivity.
+              rewrite IHc2.
+              rewrite <- seqA_sound.
+              rewrite store_store_elimination_correct; auto.
+              reflexivity.
+              rewrite IHc2. reflexivity.
+        -- destruct (String.eqb_spec x x0); simpl; subst.
+           destruct (contains x0 a0) eqn : HC; simpl.
+           rewrite IHc2. reflexivity.
+           rewrite IHc2.
+           rewrite <- seqA_sound.
+           rewrite store_store_elimination_correct; auto.
+              reflexivity.
+              rewrite IHc2. reflexivity.
+        -- destruct (String.eqb_spec x x0); simpl; subst.
+           destruct (contains x0 a0) eqn : HC; simpl.
+           rewrite IHc2. reflexivity.
+           rewrite IHc2.
+           rewrite <- seqA_sound.
+           rewrite store_store_elimination_correct; auto.
+              reflexivity.
+              rewrite IHc2. reflexivity.
+  - rewrite <- IHc1, <- IHc2. reflexivity.
+  - rewrite <- IHc. reflexivity.
+Qed.
+
+
+
+
+
+
+
+
+
+
+(** Example: using verified optimizations to prove an
+equivalence between Imp programs. *)
+
+Example opt_fact_sound :
+  <{ X := 5;
+     Z := X;
+     Y := 1;
+     while Z <> 0 do
+        Y := Y * Z;
+        Z := Z - 1
+     end }>
+    ≊
+  <{ X := 5; Z := 0; Y := 120 }>.
+Proof.
+  rewrite (optimize_sound 6).
+  cbn.
+  rewrite dead_store_elimination_correct.
+  cbn.
+  rewrite skipR_sound.
+  reflexivity.
+Qed.
+
+(* 2024-06-13 11:26 *)
