ImpShort.v
@@ -246,4 +246,4 @@ Consequently: not very extensible, hard to re-use the metatheory.
 Can we do it differently?
 *)
 
-(* 2024-06-07 10:32 *)
+(* 2024-06-13 11:26 *)
