Monads.v
@@ -1660,4 +1660,4 @@ database it must return a copy of the entire database.
     something simple, we would like our functional programs to [load] and
     [store] a single register of type [nat]. *)
 
-(* 2024-06-10 14:53 *)
+(* 2024-06-13 11:26 *)
