Further.v
@@ -32,20 +32,31 @@ Interaction Trees & Their Uses:
 - Interaction Trees [POPL 2020]
 - C4: Verified Transactional Objects [OOPSLA 2022]
 - Vellvm [ICFP 2021]
-- DeepSpec WebServer / Network Testing
+- Choice Trees: Representing Nondeterministic, Recursive, and Impure Programs in Coq [POPL 2023]
+- Semantics for Noninterference with Interaction Trees [ECOOP 2023]
+
+Free Monads / Algebraic Effects:
+
+- Papers by Matija Pretnar, Plotkin, Power (especialy Handling Algebraic Effects [CCS 2012]
 
 Monadic Reasoning:
 
-- Dijkstra Monads (For All / For Free / Forever / ...)  _Maillaird, Hrițcu, et al._
+- Dijkstra Monads (For All / For Free / Forever / ...)  _Maillaird, Hrițcu_ et al.
 
 - Formal Reasoning About Layered Monadic Interpreters  _Yoon, Zakowski, Zdancewic_ [ICFP 22]
 
 Relational Reasoning:
 
-- Simple relational correctness proofs for static analyses and program transformations [Benton]
+- Simple relational correctness proofs for static analyses and program transformations [Benton POPL 2004]
 
-- The Next 700 Relational Program Logics  _Maillaird, Hrițcu, et al._
+- The Next 700 Relational Program Logics  _Maillaird, Hrițcu_ et al
+
+Coinduction:
+
+- The power of parameterization in coinductive proof, _Hur_ et al. [POPL 13]
+
+- Anything by _Damien Pous_, but especially: Coinduction All the Qay Up
 
 *)
 
-(* 2024-06-07 10:32 *)
+(* 2024-06-13 11:26 *)
